working/composition/event_based_refinement/load_balancer/RefinementProof.v.dfy
@@ -20,20 +20,83 @@ module RefinementProof refines RefinementTheorem {
         Spec.Constants()
     }
 
+    ghost function MapClientRequests(clientRequests: seq<ClientRequest>) : seq<(int, int)>
+        decreases |clientRequests|
+        ensures |clientRequests| == |MapClientRequests(clientRequests)|
+        ensures forall i :: 0 <= i < |clientRequests| ==> MapClientRequests(clientRequests)[i] == (clientRequests[i].x, clientRequests[i].y)
+    {
+        if |clientRequests| == 0
+            then [] 
+            else [(clientRequests[0].x, clientRequests[0].y)] + MapClientRequests(clientRequests[1..])
+    }
+
+    ghost function MapClientResponses(clientResponses: seq<ClientResponse>) : seq<(int)>
+        decreases |clientResponses|
+        ensures |clientResponses| == |MapClientResponses(clientResponses)|
+        ensures forall i :: 0 <= i < |clientResponses| ==> MapClientResponses(clientResponses)[i] == clientResponses[i].sum
+    {
+        if |clientResponses| == 0
+            then [] 
+            else [clientResponses[0].sum] + MapClientResponses(clientResponses[1..])
+    }
+
     ghost function VariablesAbstraction(c: DistributedSystem.Constants, v: DistributedSystem.Variables) : Spec.Variables
 //        requires v.WF(c)
     {
-        Spec.Variables(v.hosts[0].client.req, v.hosts[0].client.resp)
+        Spec.Variables(
+            MapClientRequests(v.hosts[0].client.requests), 
+            MapClientResponses(v.hosts[0].client.responses)
+        )
+    }
+
+    ghost predicate Inv_ClientRequestMsg(c: DistributedSystem.Constants, v: DistributedSystem.Variables) 
+        requires v.WF(c)
+    {
+        forall msg :: 
+            && msg in v.network.sentMsgs 
+            && msg.ClientRequestMsg? ==> 
+            && |v.hosts[0].client.requests| > msg.request.seqNo 
+            && v.hosts[0].client.requests[msg.request.seqNo] == msg.request
+    }
+
+    ghost predicate Inv_LBRequestMsg(c: DistributedSystem.Constants, v: DistributedSystem.Variables) 
+        requires v.WF(c)
+    {
+        forall msg :: 
+            && msg in v.network.sentMsgs 
+            && msg.LBRequestMsg?  ==> 
+            && |v.hosts[0].client.requests| > msg.request.seqNo 
+            && v.hosts[0].client.requests[msg.request.seqNo] == msg.request
+    }
+
+    ghost predicate Inv_LBResponseMsg(c: DistributedSystem.Constants, v: DistributedSystem.Variables) 
+        requires v.WF(c)
+    {
+        forall msg :: 
+            && msg in v.network.sentMsgs 
+            && msg.LBResponseMsg? ==> 
+            && |v.hosts[0].client.requests| > msg.response.seqNo 
+            && v.hosts[0].client.requests[msg.response.seqNo].x + v.hosts[0].client.requests[msg.response.seqNo].y == msg.response.sum
+    }
+
+    ghost predicate Inv_ClientResponseMsg(c: DistributedSystem.Constants, v: DistributedSystem.Variables) 
+        requires v.WF(c)
+    {
+        forall msg :: 
+            && msg in v.network.sentMsgs 
+            && msg.ClientResponseMsg? ==> 
+            && |v.hosts[0].client.requests| > msg.response.seqNo 
+            && v.hosts[0].client.requests[msg.response.seqNo].x + v.hosts[0].client.requests[msg.response.seqNo].y == msg.response.sum
     }
 
     ghost predicate Inv(c: DistributedSystem.Constants, v: DistributedSystem.Variables)
     {
         && v.WF(c)
-        && (forall msg :: msg in v.network.sentMsgs && msg.ClientRequest? ==> v.hosts[0].client.req.Some? && msg == ClientRequest(v.hosts[0].client.req.value.0, v.hosts[0].client.req.value.1))
-        && (forall msg :: msg in v.network.sentMsgs && msg.LBRequest? ==> v.hosts[0].client.req.Some? && msg == LBRequest(v.hosts[0].client.req.value.0, v.hosts[0].client.req.value.1))
-        && (forall msg :: msg in v.network.sentMsgs && msg.LBResponse? ==> v.hosts[0].client.req.Some? && msg == LBResponse(v.hosts[0].client.req.value.0 + v.hosts[0].client.req.value.1))
-        && (forall msg :: msg in v.network.sentMsgs && msg.ClientResponse? ==> v.hosts[0].client.req.Some? && msg == ClientResponse(v.hosts[0].client.req.value.0 + v.hosts[0].client.req.value.1))
-    }
+        && Inv_ClientRequestMsg(c, v)
+        && Inv_LBRequestMsg(c, v)
+        && Inv_LBResponseMsg(c, v)
+        && Inv_ClientResponseMsg(c, v)
+   }
 
     lemma RefinementInit(c: DistributedSystem.Constants, v: DistributedSystem.Variables)
 //        requires DistributedSystem.Init(c, v)
