working/composition/event_based_refinement/load_balancer/Server.v.dfy
@@ -9,7 +9,7 @@ module ServerHost {
         }
     }
 
-    datatype Variables = Variables(sum: Option<int>)
+    datatype Variables = Variables(processed: set<SeqNo>)
     {
         ghost predicate WF(c: Constants) {
             true
@@ -17,16 +17,16 @@ module ServerHost {
     }
 
     ghost predicate Init(c: Constants, v: Variables) {
-        && v.sum.None?
+        && |v.processed| == 0
     }
 
     ghost predicate Compute(c: Constants, v: Variables, v': Variables, evt: Event, msgOps: MessageOps) {
         && evt.NoOp?
         && msgOps.recv.Some?
-        && msgOps.recv.value.LBRequest?
-        && msgOps.send == Some(LBResponse(msgOps.recv.value.x + msgOps.recv.value.y))
-        && v.sum.None?
-        && v'.sum == Some(msgOps.recv.value.x + msgOps.recv.value.y)
+        && msgOps.recv.value.LBRequestMsg?
+        && msgOps.recv.value.request.seqNo !in v.processed
+        && v'.processed == v.processed + { msgOps.recv.value.request.seqNo }
+        && msgOps.send == Some(LBResponseMsg(ClientResponse(msgOps.recv.value.request.seqNo, msgOps.recv.value.request.x + msgOps.recv.value.request.y)))
     }
 
     ghost predicate Next(c: Constants, v: Variables, v': Variables, evt: Event, msgOps: MessageOps)
